Meta/PermutateOr.lean
@@ -1,22 +1,18 @@
-import Meta.Resolution
-
 import Lean
-open Lean
-open Lean.Elab.Tactic Lean.Syntax Lean.Elab Lean.Expr
-open Lean.Elab.Tactic
+
+import Meta.Resolution
+import Meta.Util
+
+open Lean Elab Tactic
 
 -- TODO: find a way to remove '?' without breaking the parser
 syntax (name := permutateOr) "permutateOr" term "," ("[" term,* "]")? : tactic
 
 def parsePermuteOr : Syntax → TacticM (List Nat)
-  | `(tactic| permutateOr $_, [ $[$hs],* ]) => hs.toList.mapM stxToNat
-  | _                                      => throwError "ble"
-
-def getIthExpr : Nat → Expr → Option Expr
-  | Nat.zero, app (app (const `Or ..) t₁) _ => some t₁
-  | Nat.zero, t                             => some t -- last element in or chain
-  | i + 1,    app (app (const `Or ..) _) t₂ => getIthExpr i t₂
-  | _, _                                    => none
+  | `(tactic| permutateOr $_, [ $[$hs],* ]) =>
+    hs.toList.mapM stxToNat
+  | _ =>
+    throwError "[permutateOr]: wrong usage"
 
 @[tactic permutateOr] def evalPermutateOr : Tactic :=
   fun stx => withMainContext do
@@ -30,7 +26,7 @@ where go : List Nat → Expr → Expr → Syntax → TacticM Expr
        | (i::is), type, hyp, stx => do
          let fname ← mkIdent <$> mkFreshId
          let ithExpr ←
-           match getIthExpr i type with
+           match getIthExpr? i type with
            | some e => pure e
            | none   => throwError "invalid permutation"
          let type ← instantiateMVars (← Meta.inferType hyp)
@@ -39,11 +35,4 @@ where go : List Nat → Expr → Expr → Syntax → TacticM Expr
            let ctx ← getLCtx
            let hyp' := (ctx.findFromUserName? fname.getId).get!.toExpr
            go is type hyp' stx
-
-
-example : A ∨ B ∨ C ∨ D ∨ E → True := by
-  intro h
-  trivial
-  /- permutateOr h, [2, 1, 3, 4, 0] -/
-  /- trivial -/
 
